correcting silent_reachable_set(p) definition

LTS.thy
@@ -60,7 +60,17 @@ definition weakly_trace_preordered (infix "\<lesssim>WT" 60) where
 definition weakly_trace_equivalent (infix "\<simeq>WT" 60) where
 "p \<simeq>WT q \<equiv> p \<lesssim>WT q \<and> q \<lesssim>WT p"
 
-abbreviation silent_reachable_set (infix "\<Zsurj>S" 80) where "P \<Zsurj>S Q \<equiv> \<forall>p \<in> P. \<forall>q \<in> Q. p \<Zsurj> q"
+
+abbreviation silent_reachable_setp (infix "\<Zsurj>S" 80) where
+  "P \<Zsurj>S Q \<equiv> ((\<forall>q \<in> Q. \<exists>p \<in> P. p \<Zsurj> q) \<and> (\<forall>p \<in> P. \<forall>q. p \<Zsurj> q \<longrightarrow> q \<in> Q))"
+
+definition silent_reachable_set :: "'s set \<Rightarrow> 's set" where
+  "silent_reachable_set P \<equiv> { q . \<exists>p \<in> P. p \<Zsurj> q }"
+
+lemma sreachable_set_is_sreachable: "P \<Zsurj>S (silent_reachable_set P)"
+  using silent_reachable_set_def by auto
+
+
 abbreviation non_tau_step_set ("_ \<mapsto>aS _ _" [70,70,70] 80) where "P \<mapsto>aS \<alpha> Q \<equiv> \<forall>p \<in> P. \<forall>q \<in> Q. p \<mapsto>a \<alpha> q"
 
 end (* locale LTS_Tau *)
